close admits

theories/playground/language.v
@@ -12,7 +12,8 @@ Class Language := {
 
 
 Notation pool := (list (expr * expr)).
-Notation delays := (list nat).
+Notation trace := (list nat).
+Notation delays := (gmap nat nat).
 
 (* Language Setup *)
 Notation "P '.(tgt)'" := (P.*1) (at level 5).
@@ -78,13 +79,12 @@ Section language_setup.
       i = length T_l →
       pool_step (T_l ++ e :: T_r) i (T_l ++ e' :: T_r ++ T_f).
 
-  Inductive pool_steps : list expr → gset nat → list expr → Prop :=
-    | pool_no_steps T: pool_steps T ∅ T
-    | pool_do_steps T T' T'' i I J:
+  Inductive pool_steps : list expr → trace → list expr → Prop :=
+    | pool_no_steps T: pool_steps T [] T
+    | pool_do_steps T T' T'' i I:
       pool_step T i T' →
       pool_steps T' I T'' →
-      J ≡ I ∪ {[i]} →
-      pool_steps T J T''.
+      pool_steps T (i:: I) T''.
 
 
   Lemma pool_step_iff T i T':
@@ -111,10 +111,9 @@ Section language_setup.
 
   Lemma pool_steps_single T i T':
     pool_step T i T' →
-    pool_steps T {[i]} T'.
+    pool_steps T [i] T'.
   Proof.
-    intros Hstep; econstructor; [eauto|constructor|].
-    set_solver.
+    intros Hstep; econstructor; [eauto|constructor].
   Qed.
 
   Lemma pool_step_value_preservation e T i j T':
@@ -140,11 +139,11 @@ Section language_setup.
     induction 1; eauto using pool_step_value_preservation.
   Qed.
 
-  Lemma no_forks_pool_steps e e' e'' i T:
+  (* Lemma no_forks_pool_steps e e' e'' i T:
     no_fork e e' →
     no_forks e' e'' →
     T !! i = Some e →
-    pool_steps T {[i]} (<[i := e'']> T).
+    pool_steps T [i] (<[i := e'']> T).
   Proof.
     intros Hstep Hsteps.
     revert e T Hstep.
@@ -158,76 +157,79 @@ Section language_setup.
       + rewrite -(list_insert_insert T i e''' e'). eapply IH; eauto.
         eapply list_lookup_insert, lookup_lt_Some, Hlook.
       + set_solver.
-  Qed.
+  Qed. *)
 
-  Lemma pool_steps_set_morph T T' I J:
-    pool_steps T I T' →
-    I ≡ J →
-    pool_steps T J T'.
-  Proof.
-    by intros ? ->%leibniz_equiv.
-  Qed.
-
-  Lemma pool_steps_trans T T' T'' I I' J:
+  Lemma pool_steps_trans T T' T'' I I':
     pool_steps T I T' →
     pool_steps T' I' T'' →
-    I ∪ I' ≡ J →
-    pool_steps T J T''.
+    pool_steps T (I ++ I') T''.
   Proof.
-    induction 1 in J.
-    - intros Hsteps Heq; eapply pool_steps_set_morph; first apply Hsteps. set_solver.
-    - intros Hsteps Heq. econstructor; eauto. set_solver.
+    induction 1.
+    - by rewrite left_id.
+    - intros; simpl; econstructor; eauto.
   Qed.
 
 
   (* an expression is active in a thread pool,
     if it is not a value *)
-    Inductive fair_pool_step : list expr → list nat → nat → list expr → list nat → Prop :=
-      take_fair_step i T T' D D':
-      pool_step T i T' →
-      (∀ j n, j ≠ i → D !! j = Some n → ∃ n', n = S n' ∧ D' !! j = Some n') →
-      fair_pool_step T D i T' D'.
 
-    Lemma fair_pool_step_iff T D i T' D':
-      fair_pool_step T D i T' D' ↔
-        pool_step T i T' ∧ (∀ j n, j ≠ i → D !! j = Some n → ∃ n', n = S n' ∧ D' !! j = Some n').
-    Proof.
-      split; destruct 1; eauto 10 using take_fair_step.
-    Qed.
+  Definition active_threads T :=
+    list_to_set (C := gset nat) (fmap fst (filter (λ '(i, e), ¬ val e) (imap pair T))).
 
-    Lemma fair_pool_step_inv T D i T' D':
-      fair_pool_step T D i T' D' →
-        ∃ e e' T_f, step e e' T_f ∧
-        T !! i = Some e ∧
-        T' = <[i := e']> T ++ T_f ∧
-        (∀ j n, j ≠ i → D !! j = Some n → ∃ n', n = S n' ∧ D' !! j = Some n').
-    Proof.
-      destruct 1 as [i T T' D D' Pool Hdecr].
-      eapply pool_step_iff in Pool as (e & e' & T_f & Hstep & Hlook & Hupd).
-      eauto 10.
-    Qed.
+  Lemma active_threads_spec T i:
+    i ∈ active_threads T ↔ ∃ e, T !! i = Some e ∧ ¬ val e.
+  Proof.
+    rewrite /active_threads elem_of_list_to_set elem_of_list_fmap.
+    split.
+    - intros [[i' e] [-> Hlook]]; simpl.
+      eapply elem_of_list_filter in Hlook as [? Hlook].
+      eapply elem_of_lookup_imap in Hlook as (? & ? & Heq & ?).
+      injection Heq as ??; subst. eexists; split; eauto.
+    - intros [e [Hlook Hval]]. exists (i, e).
+      split; first done. eapply elem_of_list_filter.
+      split; first done. eapply elem_of_lookup_imap.
+      eexists _, _. split; done.
+  Qed.
+
+  Definition delays_for T D :=
+    ∀ i, i ∈ active_threads T → is_Some (D !! i).
 
 
-    Definition active_threads T :=
-      list_to_set (C := gset nat) (fmap fst (filter (λ '(i, e), ¬ val e) (imap pair T))).
+  Inductive fair_pool_step : list expr → delays → nat → list expr → delays → Prop :=
+    take_fair_step i T T' D D':
+    pool_step T i T' →
+    (∀ j n, j ≠ i → D !! j = Some n → ∃ n', n = S n' ∧ D' !! j = Some n') →
+    fair_pool_step T D i T' D'.
 
-    Lemma active_threads_spec T i:
-      i ∈ active_threads T ↔ ∃ e, T !! i = Some e ∧ ¬ val e.
-    Proof.
-      rewrite /active_threads elem_of_list_to_set elem_of_list_fmap.
-      split.
-      - intros [[i' e] [-> Hlook]]; simpl.
-        eapply elem_of_list_filter in Hlook as [? Hlook].
-        eapply elem_of_lookup_imap in Hlook as (? & ? & Heq & ?).
-        injection Heq as ??; subst. eexists; split; eauto.
-      - intros [e [Hlook Hval]]. exists (i, e).
-        split; first done. eapply elem_of_list_filter.
-        split; first done. eapply elem_of_lookup_imap.
-        eexists _, _. split; done.
-    Qed.
+  (* an expression is active in a thread pool,
+  if it is not a value *)
+  Inductive fair_pool_steps : list expr → delays → trace → list expr → delays → Prop :=
+  | fair_pool_no_steps T (D: delays): delays_for T D → fair_pool_steps T D [] T D
+  | fair_pool_do_steps T T' T'' (D D' D'': delays) i I:
+    delays_for T D →
+    fair_pool_step T D i T' D' →
+    fair_pool_steps T' D' I T'' D'' →
+    fair_pool_steps T D (i :: I) T'' D''.
 
-    Definition delays_for T D :=
-      ∀ i, i ∈ active_threads T → is_Some (D !! i).
+  Lemma fair_pool_step_iff T D i T' D':
+    fair_pool_step T D i T' D' ↔
+      pool_step T i T' ∧ (∀ j n, j ≠ i → D !! j = Some n → ∃ n', n = S n' ∧ D' !! j = Some n').
+  Proof.
+    split; destruct 1; eauto 10 using take_fair_step.
+  Qed.
+
+  Lemma fair_pool_step_inv T D i T' D':
+    fair_pool_step T D i T' D' →
+      ∃ e e' T_f, step e e' T_f ∧
+      T !! i = Some e ∧
+      T' = <[i := e']> T ++ T_f ∧
+      (∀ j n, j ≠ i → D !! j = Some n → ∃ n', n = S n' ∧ D' !! j = Some n').
+  Proof.
+    destruct 1 as [i T T' D D' Pool Hdecr].
+    eapply pool_step_iff in Pool as (e & e' & T_f & Hstep & Hlook & Hupd).
+    eauto 10.
+  Qed.
+
 
 
   CoInductive fair_div T D : Prop :=
@@ -237,15 +239,19 @@ Section language_setup.
     fair_div T' D' →
     fair_div T D.
 
-  Inductive val_or_step : list expr → gset nat → list expr → Prop :=
-    | val_or_step_values T O:
-      (∀ i, i ∈ O → ∃ e, T !! i = Some e ∧ val e) → val_or_step T O T
-    | val_or_step_step I O T T' T'':
-        pool_steps T I T' → val_or_step T' (O ∖ I) T'' → val_or_step T O T''.
+
+  CoInductive fair_div_tc T D : Prop :=
+  | fair_div_tc_step I T' D':
+    I ≠ [] →
+    fair_pool_steps T D I T' D' →
+    fair_div_tc T' D' →
+    fair_div_tc T D.
+
 
   CoInductive fair_div_alt T : Prop :=
-    fair_div_alt_step T':
-    val_or_step T (threads T) T' →
+    fair_div_alt_step T' I:
+    pool_steps T I T' →
+    ∅ ⊂ active_threads T ⊆ list_to_set I →
     fair_div_alt T' →
     fair_div_alt T.
 
@@ -281,12 +287,12 @@ Section language_setup.
   Proof. by destruct 1. Qed.
 
   Lemma fair_div_active_threads_steps T D:
-    fair_div T D → ∃ T' D' O, active_threads T ⊆ O ∧ fair_div T' D' ∧ pool_steps T O T'.
+    fair_div T D → ∃ T' D' O, active_threads T ⊆ list_to_set O ∧ fair_div T' D' ∧ pool_steps T O T'.
   Proof.
-    enough (∀ O T D, O ⊆ active_threads T → fair_div T D → ∃ T' D' O', O ⊆ O' ∧ fair_div T' D' ∧ pool_steps T O' T') by eauto.
+    enough (∀ O T D, O ⊆ active_threads T → fair_div T D → ∃ T' D' O', O ⊆ list_to_set O' ∧ fair_div T' D' ∧ pool_steps T O' T') by eauto.
     clear T D; intros O; induction (set_wf O) as [O _ IHO]; intros T D Hsub Hfair.
     destruct (decide (O ≡ ∅)) as [->%leibniz_equiv|[i Hi]%set_choose].
-    - exists T, D, ∅. do 2 (split; first done). constructor.
+    - exists T, D, []. do 2 (split; first done). constructor.
     - assert (delays_for T D) as Hdel by by destruct Hfair.
       assert (is_Some (D !! i)) as [d HD] by eapply Hdel, Hsub, Hi.
       revert T D Hsub Hfair Hdel HD. induction (lt_wf d) as [d _ IHd].
@@ -297,7 +303,7 @@ Section language_setup.
         * by set_solver.
         * etrans; last by apply active_threads_step. set_solver.
         * apply Hfair.
-        * exists T'', D'', (O' ∪ {[j]}); split.
+        * exists T'', D'', (j :: O'); split.
          { intros k Hk; destruct (decide (k = j)); set_solver. }
           split; first done.
           econstructor; eauto.
@@ -309,26 +315,250 @@ Section language_setup.
         * eauto.
         * by eapply fair_div_delays.
         * done.
-        * exists T'', D'', (O' ∪ {[j]}); split.
+        * exists T'', D'', (j :: O'); split.
           { intros k Hk; destruct (decide (k = j)); set_solver. }
           split; first done.
           econstructor; eauto.
   Qed.
 
 
-  Lemma fair_div_foo T D:
+  Lemma fair_div_has_active T D:
+    fair_div T D → ∅ ⊂ active_threads T.
+  Proof.
+    destruct 1 as [j T' D' Hfair Hdel ?].
+    enough (j ∈ active_threads T) by set_solver.
+    eapply fair_pool_step_inv in Hfair as (e & e' & T_f & Step & Hlook & Hinsert & Hdecr).
+    eapply active_threads_spec. exists e.
+    split; first done. pose proof val_no_step. naive_solver.
+  Qed.
+
+  Lemma fair_div_fair_div_alt T D:
     fair_div T D → fair_div_alt T.
   Proof.
     revert T D; cofix IH; intros T D Hfair.
+    eapply fair_div_has_active in Hfair as Hact.
     eapply fair_div_active_threads_steps in Hfair as (T' & D' & O & Hsub & Hfair' & Hsteps).
-    apply (fair_div_alt_step T T'); last eauto.
-    econstructor; eauto.
-    constructor. intros i [Hi Ho]%elem_of_difference.
-    eapply threads_spec in Hi as [e Hlook].
-    destruct (decide (val e)).
-    - exists e; split; last done. by eapply pool_steps_value_preservation.
-    - exfalso. eapply Ho, Hsub, active_threads_spec. eauto 10.
+    apply (fair_div_alt_step T T' O); eauto.
   Qed.
 
+
+
+  Lemma pool_step_to_fair_pool_step T i T' D:
+    pool_step T i T' → fair_pool_step T (<[i:=0]> (S <$> D)) i T' D.
+  Proof.
+    intros Hstep; eapply fair_pool_step_iff.
+    split; first done.
+    intros j n Hne. rewrite lookup_insert_ne // lookup_fmap.
+    destruct (D !! j); simpl; naive_solver.
+  Qed.
+
+  Fixpoint delays_for_trace I D :=
+    match I with
+    | nil => D
+    | i :: I' => <[i := 0]> (S <$> delays_for_trace I' D)
+    end.
+
+  Definition active_only T D := filter (λ '(i, n), i ∈ active_threads T) D.
+
+  Notation trace_delays T I D := (active_only T (delays_for_trace I D)).
+
+  Lemma delays_for_trace_oblivious_single i I D1 D2:
+    i ∈ I → delays_for_trace I D1 !! i = delays_for_trace I D2 !! i.
+  Proof.
+    induction 1 as [i|i j I Hel IH]; simpl.
+    - by rewrite !lookup_insert.
+    - destruct (decide (i = j)); first (subst; by rewrite !lookup_insert).
+      by rewrite !lookup_insert_ne //= !lookup_fmap IH.
+  Qed.
+
+
+  Lemma delays_for_trace_oblivious T I D1 D2:
+    active_threads T ⊆ list_to_set I → trace_delays T I D1 = trace_delays T I D2.
+  Proof.
+    intros Hact; eapply map_filter_strong_ext.
+    intros i d.
+    split; intros [Hact' Hdel]; (split; first done);
+    erewrite delays_for_trace_oblivious_single; set_solver.
+  Qed.
+
+
+  Lemma delays_for_active_only T D:
+    delays_for T (active_only T D) ↔ delays_for T D.
+  Proof.
+    split; intros Hdel j Hj; destruct (Hdel j Hj) as [d HD];
+      exists d.
+    - eapply map_filter_lookup_Some_1_1, HD.
+    - eapply map_filter_lookup_Some; eauto.
+  Qed.
+
+  Lemma pool_step_delays_for T i T' D:
+    pool_step T i T' →
+    delays_for T' D →
+    delays_for T (<[i := 0]> (S <$> D)).
+  Proof.
+    intros Hstep Hdel. intros j Hj. destruct (decide (i = j)).
+    { subst; rewrite lookup_insert; eauto. }
+    rewrite lookup_insert_ne // lookup_fmap fmap_is_Some.
+    eapply Hdel, active_threads_step; eauto.
+    set_solver.
+  Qed.
+
+  Lemma pool_steps_delays_for T I T' D:
+    pool_steps T I T' →
+    delays_for T' D →
+    delays_for T (delays_for_trace I D).
+  Proof.
+    induction 1 as [T|T T' T'' i I Hstep Hsteps IH];
+      simpl; eauto using pool_step_delays_for.
+  Qed.
+
+  Lemma pool_steps_to_fair_pool_steps T I T' D:
+    pool_steps T I T' →
+    delays_for T' D →
+    fair_pool_steps T (delays_for_trace I D) I T' D.
+  Proof.
+    induction 1 as [T|T T' T'' i I Hstep Hsteps IH]; simpl.
+    - by constructor.
+    - econstructor; eauto using pool_step_to_fair_pool_step.
+      eauto using pool_step_delays_for, pool_steps_delays_for.
+  Qed.
+
+  Lemma fair_pool_active_only T D i T' D':
+    fair_pool_step T D i T' D' →
+    fair_pool_step T (active_only T D) i T' (active_only T' D').
+  Proof.
+    destruct 1 as [i T T' D D' Hstep Hdecr].
+    econstructor; first done.
+    intros j d Hne Hactive. eapply map_filter_lookup_Some in Hactive as [HD Hact].
+    destruct (Hdecr j d  Hne HD) as (d' & -> & HD').
+    exists d'; split; first done.
+    eapply map_filter_lookup_Some; split; first done.
+    eapply active_threads_step; eauto.
+    set_solver.
+  Qed.
+
+
+  Lemma fair_pool_steps_active_only T D I T' D':
+    fair_pool_steps T D I T' D' →
+    fair_pool_steps T (active_only T D) I T' (active_only T' D').
+  Proof.
+    induction 1 as [T|T T' T'' D D' D'' i I Hstep Hsteps IH]; simpl.
+    - constructor; by eapply delays_for_active_only.
+    - econstructor; eauto using fair_pool_active_only.
+      by eapply delays_for_active_only.
+  Qed.
+
+  Lemma fair_div_alt_trace T:
+    fair_div_alt T → ∃ I T', ∅ ⊂ active_threads T ⊆ list_to_set I ∧ pool_steps T I T' ∧ fair_div_alt T'.
+  Proof.
+    destruct 1 as [T' I Hstep Hsub Hfair]; eauto 10.
+  Qed.
+
+  Require Import Coq.Logic.Epsilon.
+  Lemma fair_div_alt_trace_strong T:
+    fair_div_alt T → { I | ∃ T', ∅ ⊂ active_threads T ⊆ list_to_set I ∧ pool_steps T I T' ∧ fair_div_alt T' }.
+  Proof.
+    intros Hdiv. eapply constructive_indefinite_description, fair_div_alt_trace, Hdiv.
+  Qed.
+
+  Definition fair_div_alt_delays T (Div: fair_div_alt T) :=
+      active_only T (delays_for_trace (proj1_sig (fair_div_alt_trace_strong T Div)) ∅).
+
+  Lemma delays_for_delays_for_trace T T' I D:
+    active_threads T ⊆ list_to_set I → pool_steps T I T' → delays_for T (delays_for_trace I D).
+  Proof.
+    intros Hsub Hsteps. eapply delays_for_active_only.
+    rewrite (delays_for_trace_oblivious _ _ _ (gset_to_gmap 0 (threads T'))); last done.
+    eapply delays_for_active_only, pool_steps_delays_for; first done.
+    intros j Hj. eapply active_threads_spec in Hj as (e & Hlook & _).
+    exists 0. eapply lookup_gset_to_gmap_Some; split; last done.
+    eapply threads_spec; eauto.
+  Qed.
+
+
+  Lemma fair_pool_steps_delays_for_start T D I T' D':
+    fair_pool_steps T D I T' D' → delays_for T D.
+  Proof.
+    destruct 1; done.
+  Qed.
+
+  Lemma fair_pool_steps_delays_for_end T D I T' D':
+    fair_pool_steps T D I T' D' → delays_for T' D'.
+  Proof.
+    induction 1; eauto.
+  Qed.
+
+
+  Lemma fair_div_alt_inv T (Div: fair_div_alt T):
+    ∃ T' (Div': fair_div_alt T') I,
+      I ≠ [] ∧
+      fair_pool_steps T (fair_div_alt_delays T Div) I T' (fair_div_alt_delays T' Div').
+  Proof.
+    rewrite /fair_div_alt_delays.
+    destruct (fair_div_alt_trace_strong T) as (I & T' & Hsub & Hsteps & Div'); simpl.
+    exists T', Div', I. split.
+    - intros ->; set_solver.
+    - remember (delays_for_trace (proj1_sig (fair_div_alt_trace_strong T' Div')) ∅) as D'.
+      rewrite (delays_for_trace_oblivious _ _ ∅ D'); last apply Hsub.
+      eapply fair_pool_steps_active_only, pool_steps_to_fair_pool_steps; first done.
+      (* TODO: this part of the proof is odd, there should be better factoring *)
+      subst D'.
+      destruct (fair_div_alt_trace_strong) as (I' & T'' & Hsub' & Hsteps' & Div''); simpl.
+      eapply delays_for_delays_for_trace; eauto. apply Hsub'.
+  Qed.
+
+
+  Lemma fair_div_insert_steps T D I T' D':
+    fair_pool_steps T D I T' D' → fair_div T' D' → fair_div T D.
+  Proof.
+    induction 1 as [T|T T' T'' D D' D'' i I Hstep Hsteps IH]; eauto.
+    intros Hdiv; econstructor; eauto.
+  Qed.
+
+
+  Lemma fair_pool_steps_concat T D I T' D' J T''' D''':
+    fair_pool_steps T D I T' D' → fair_pool_steps T' D' J T''' D''' →  fair_pool_steps T D (I ++ J) T''' D'''.
+  Proof.
+    induction 1 as [T|T T' T'' D D' D'' i I Hdel Hstep Hsteps IH]; simpl; eauto.
+    intros Hsteps'%IH. econstructor; eauto.
+  Qed.
+
+  Lemma fair_div_tc_insert_steps T D I T' D':
+    fair_pool_steps T D I T' D' → fair_div_tc T' D' → fair_div_tc T D.
+  Proof.
+    intros Hsteps; destruct 1 as [J T''' D''' Hne Hsteps'' Hdiv''].
+    econstructor; [|by eapply fair_pool_steps_concat|done].
+    destruct I; simpl; naive_solver.
+  Qed.
+
+  Lemma fair_div_alt_fair_div_tc T:
+    fair_div_alt T → ∃ D, fair_div_tc T D.
+  Proof.
+    intros Div. exists (fair_div_alt_delays T Div).
+    revert T Div; cofix IH; intros T Div.
+    destruct (fair_div_alt_inv T Div) as (T' & Div' & I & Hne & Hsteps).
+    destruct I as [|i I]; first naive_solver.
+    inversion Hsteps as [|? T_mid ?? D_mid ? ? ? Hdel Hstep Hsteps']; subst.
+    econstructor; eauto.
+  Qed.
+
+  Lemma fair_div_tc_fair_div T D:
+    fair_div_tc T D → fair_div T D.
+  Proof.
+    revert T D; cofix IH; intros T D.
+    destruct 1 as [I T' D' Hne Hsteps Hdiv].
+    destruct Hsteps as [|T T' T'' D D' D'' i I Hdel Hstep Hsteps]; first naive_solver.
+    econstructor; eauto. eapply IH, fair_div_tc_insert_steps, Hdiv. done.
+  Qed.
+
+
+  Theorem fair_div_iff T:
+    fair_div_alt T ↔ (∃ D, fair_div T D).
+  Proof.
+    split.
+    - intros [D HD]%fair_div_alt_fair_div_tc.
+      eapply fair_div_tc_fair_div in HD; by exists D.
+    - intros [D HD]. by eapply fair_div_fair_div_alt.
+  Qed.
 
 End language_setup.
